src/library/tactic/apply_tactic.h
@@ -7,7 +7,33 @@ Author: Leonardo de Moura
 #pragma once
 #include "library/tactic/tactic_state.h"
 namespace lean {
-optional<tactic_state> apply(type_context & ctx, bool add_all, bool use_instances, expr const & e, tactic_state const & s);
+/*
+inductive new_goals
+| non_dep_first | non_dep_only | all
+*/
+enum class new_goals_kind { NonDepFirst, NonDepOnly, All };
+/*
+structure apply_cfg :=
+(md            := semireducible)
+(approx        := tt)
+(new_goals     := new_goals.non_dep_first)
+(instances     := tt)
+(auto_param    := tt)
+(opt_param     := tt)
+*/
+struct apply_cfg {
+    transparency_mode m_mode{transparency_mode::Semireducible};
+    bool              m_approx{true};
+    new_goals_kind    m_new_goals{new_goals_kind::NonDepFirst};
+    bool              m_instances{true};
+    bool              m_auto_param{true};
+    bool              m_opt_param{true};
+    apply_cfg() {}
+    apply_cfg(vm_obj const & cfg);
+};
+optional<tactic_state> apply(type_context & ctx, expr const & e, apply_cfg const & cfg, tactic_state const & s);
+/* For backward compatibility */
+optional<tactic_state> apply(type_context & ctx, bool all, bool use_instances, expr const & e, tactic_state const & s);
 void initialize_apply_tactic();
 void finalize_apply_tactic();
 }
