library/init/meta/relation_tactics.lean
@@ -14,7 +14,7 @@ do tgt   ← target,
    env   ← get_env,
    let r := get_app_fn tgt,
    match (op_for env (const_name r)) with
-   | (some refl) := do r ← mk_const refl, apply_core r {md := md} >> return ()
+   | (some refl) := do r ← mk_const refl, apply_core r {md := md, new_goals := new_goals.non_dep_only} >> return ()
    | none        := fail $ tac_name ++ " tactic failed, target is not a relation application with the expected property."
    end
 
